time_strat_liquidity/Monotonicity.v
@@ -1,0 +1,299 @@
+Require Import Monads.
+Require Import Blockchain.
+Require Import Containers.
+Require Import Serializable.
+Require Import PArith.
+Require Import Extras.
+Require Import BoundedN.
+Require Import BuildUtils.
+Require Import FMapList.
+Require Import RecordUpdate.
+Require Import Automation.
+Require Import ContractCommon.
+Require Import ResultMonad.
+Require Import InterContractCommunication.
+Require Import ChainedList.
+Require Import TimeStratModel.
+From Coq Require Import List.
+From Coq Require Import Bool.
+From Coq Require Import ZArith.
+From Coq Require Import Arith.
+From Coq Require Import String.
+From Coq Require Import Lia.
+Import RecordSetNotations.
+From Coq Require Import Permutation.
+Import ListNotations.
+Section Monotonicity.
+  Context {BaseTypes : ChainBase}.
+  Variable miner_address : Address.
+  Hypothesis miner_always_eoa : address_is_contract miner_address = false.
+  Global Definition miner_reward := 10%Z.
+
+  Notation "trace( from , to )" := (TransitionTrace miner_address from to)(at level 10).
+
+  Definition acts_subset (acts1 acts2 : list Action) : Prop :=
+    incl acts1 acts2. 
+
+  Definition acts_subset_time (acts1 acts2 : list Action) : Prop :=
+  (acts_subset acts1 acts2 ) /\ 
+  (forall a, is_wait_act a = true -> 
+              In a acts2 -> 
+              In a acts1).
+
+  Definition strat_subset 
+              (addrs1 : list Address)
+              (delta1 : strat miner_address addrs1) 
+              (addrs2 : list Address) 
+              (delta2 : strat miner_address addrs1) 
+    s0: Prop :=
+    forall s tr,
+        acts_subset
+        (packe miner_address (delta1 s0 s tr))
+        (packe miner_address (delta2 s0 s tr)). 
+
+  Definition strat_subset_time 
+    (addrs1 : list Address)
+    (delta1 : strat miner_address addrs1) 
+    (addrs2 : list Address) 
+    (delta2 : strat miner_address addrs1) 
+    s0: Prop :=
+    forall s tr,
+        acts_subset_time
+        (packe miner_address (delta1 s0 s tr))
+        (packe miner_address (delta2 s0 s tr)).
+
+  Lemma in_empty_false : forall (A : Type) (x : A), ~ In x [].
+    Proof.
+      intros A x H4.
+      inversion H4. (* 空列表中不可能有元素，因此直接矛盾。 *)
+    Qed.
+
+  Lemma in_nonempty_to_empty_contradiction : forall (A : Type) (a : A) (l : list A),
+    (forall x, In x (a :: l) -> In x []) -> False.
+  Proof.
+    intros A a l H4.
+    (* 选择一个具体的元素 a，它在 a :: l 中。 *)
+    specialize (H4 a).
+    simpl in H4.
+    destruct H4.
+    eauto.
+  Qed.
+
+  Lemma stratDrive_subset:
+    forall s0 s s' tr tr' delta_usr1 addrs_usr1 delta_usr2 addrs_usr2,
+      strat_subset addrs_usr2 delta_usr2 addrs_usr1 delta_usr1  s0 ->
+      stratDrive miner_address addrs_usr2 delta_usr2 s0 s tr s' tr' ->
+      stratDrive miner_address addrs_usr1 delta_usr1 s0 s tr s' tr'.
+  Proof.
+    unfold stratDrive.
+    unfold strat_subset.
+    unfold acts_subset.
+    intros.
+    decompose_exists.
+    destruct_and_split. 
+    specialize(H s tr).
+    exists x, x0 , x1.
+    split.
+    eauto.
+    destruct (packe miner_address (delta_usr2 s0 s tr)).
+    inversion H1.
+    eauto.
+    eauto.
+  Qed.
+
+  Lemma stratDrive_subset_time:
+    forall s0 s s' tr tr' delta_usr1 addrs_usr1 delta_usr2 addrs_usr2,
+      strat_subset_time addrs_usr2 delta_usr2 addrs_usr1 delta_usr1  s0 ->
+      stratDrive miner_address addrs_usr2 delta_usr2 s0 s tr s' tr' ->
+      stratDrive miner_address addrs_usr1 delta_usr1 s0 s tr s' tr'.
+  Proof.
+    unfold strat_subset_time.
+    unfold acts_subset_time.
+    intros.
+    decompose_exists.
+    destruct_and_split. 
+    specialize(H s tr).
+    destruct_and_split.
+    unfold stratDrive  in H0.
+    decompose_exists.
+    destruct_and_split.
+    exists x, x0 , x1.
+    split.
+    eauto.
+    destruct (packe miner_address (delta_usr2 s0 s tr)).
+    inversion H0.
+    eauto.
+  Qed.
+
+  Lemma multiStratDrive_subset:
+    forall s0 s s' tr tr' delta_usr1 addrs_usr1 delta_usr2 addrs_usr2 n,
+      strat_subset delta_usr2 addrs_usr2 delta_usr1 addrs_usr1 s0 ->
+      multiStratDrive miner_address delta_usr2 addrs_usr2 s0 s tr s' tr' n ->
+      multiStratDrive miner_address delta_usr1 addrs_usr1 s0 s tr s' tr' n.
+  Proof.
+    intros.
+    induction H0.
+    - eapply MS_Refl.
+    - eapply stratDrive_subset in H1;eauto.
+      eapply MS_Step;eauto.
+  Qed.
+
+  Lemma multiStratDrive_subset_time:
+    forall s0 s s' tr tr' delta_usr1 addrs_usr1 delta_usr2 addrs_usr2 n,
+      strat_subset_time delta_usr2 addrs_usr2 delta_usr1 addrs_usr1 s0 ->
+      multiStratDrive miner_address delta_usr2 addrs_usr2 s0 s tr s' tr' n ->
+      multiStratDrive miner_address delta_usr1 addrs_usr1 s0 s tr s' tr' n.
+  Proof.
+    intros.
+    induction H0.
+    - eapply MS_Refl.
+    - eapply stratDrive_subset_time in H1;eauto.
+      eapply MS_Step;eauto.
+  Qed.
+
+  Lemma interleavedExecution_mono_incl_usr_unchanging (addrs_usr: list Address) (delta_usr : strat miner_address addrs_usr)  (addrs_env1: list Address) (delta_env1 : strat miner_address addrs_env1) (addrs_env2: list Address) (delta_env2 : strat miner_address addrs_env2) :
+    forall s0 s' flag tr tr',
+      strat_subset addrs_env1 delta_env1 addrs_env2 delta_env2  s0 ->
+      interleavedExecution miner_address addrs_usr delta_usr addrs_env1 delta_env1  s0 s0 tr flag s' tr' ->
+      interleavedExecution miner_address addrs_usr delta_usr addrs_env2 delta_env2 s0 s0 tr flag s' tr'.
+  Proof.
+    intros * Hsbt_delta Hrc_itv.
+    induction Hrc_itv;eauto;try intuition.
+    - eapply IS_Refl.
+    - eapply (IS_Wait_Step_Once miner_address addrs_usr delta_usr addrs_env2 delta_env2 s0 s0 tr flag s' tr' s'' tr'' a1 a2);eauto.
+      unfold strat_subset in Hsbt_delta.
+      specialize (Hsbt_delta s' tr').
+      unfold acts_subset in Hsbt_delta.
+      intuition.
+    - eapply ISE_Step;eauto.
+      pose proof Hsbt_delta as Hst.
+      unfold strat_subset in Hsbt_delta.
+      specialize(Hsbt_delta  s' tr').
+      unfold acts_subset in Hsbt_delta.
+      destruct (delta_env1 s0 s' tr') eqn : He;try congruence.
+      intuition.
+      eapply multiStratDrive_subset;eauto.
+      eapply multiStratDrive_subset;eauto.
+    - eapply ISE_Turn_Step;eauto.
+      unfold strat_subset in Hsbt_delta.
+      specialize (Hsbt_delta s' tr').
+      unfold acts_subset in Hsbt_delta.
+      intuition.
+    - eapply ISU_Step;eauto.
+    - eapply ISU_Turn_Step;eauto.
+  Qed.
+
+  Lemma interleavedExecution_mono_incl_usr_unchanging_time (addrs_usr: list Address) (delta_usr : strat miner_address addrs_usr)  (addrs_env1: list Address) (delta_env1 : strat miner_address addrs_env1) (addrs_env2: list Address) (delta_env2 : strat miner_address addrs_env2) :
+    forall s0 s' flag tr tr',
+      strat_subset_time addrs_env1 delta_env1 addrs_env2 delta_env2  s0 ->
+      interleavedExecution miner_address addrs_usr delta_usr addrs_env1 delta_env1  s0 s0 tr flag s' tr' ->
+      interleavedExecution miner_address addrs_usr delta_usr addrs_env2 delta_env2 s0 s0 tr flag s' tr'.
+  Proof.
+    intros *  Hsbt_delta Hrc_itv.
+    induction Hrc_itv;eauto;try intuition.
+    - eapply IS_Refl.
+    - eapply (IS_Wait_Step_Once miner_address addrs_usr delta_usr addrs_env2 delta_env2 s0 s0 tr flag s' tr' s'' tr'' a1 a2);eauto.
+      unfold strat_subset_time in Hsbt_delta.
+      specialize (Hsbt_delta s' tr').
+      unfold acts_subset_time in Hsbt_delta.
+      destruct Hsbt_delta as [Hsbt_delta _].
+      unfold acts_subset in Hsbt_delta.
+      intuition.
+    - eapply ISE_Step;eauto.
+      pose proof Hsbt_delta as Hst.
+      unfold strat_subset_time in Hsbt_delta.
+      specialize (Hsbt_delta s' tr').
+      unfold acts_subset_time in Hsbt_delta.
+      destruct Hsbt_delta as [Hsbt_delta _].
+      unfold acts_subset in Hsbt_delta.
+      destruct (delta_env1 s0 s' tr') eqn : He;try congruence.
+      intuition.
+      eapply multiStratDrive_subset_time;eauto.
+      eapply multiStratDrive_subset_time;eauto.
+    - eapply ISE_Turn_Step;eauto.
+      unfold strat_subset_time in Hsbt_delta.
+      specialize (Hsbt_delta s' tr').
+      unfold acts_subset_time in Hsbt_delta.
+      destruct Hsbt_delta as [Hsbt_delta _].
+      unfold acts_subset in Hsbt_delta.
+      intuition.
+    - eapply ISU_Step;eauto.
+    - eapply ISU_Turn_Step;eauto.
+  Qed.
+
+  Lemma userLiquidatesNSteps_incl_usr_unchanging (addrs_usr: list Address) (delta_usr : strat miner_address addrs_usr)  (addrs_env1: list Address) (delta_env1 : strat miner_address addrs_env1) (addrs_env2: list Address) (delta_env2 : strat miner_address addrs_env2) :
+    forall s0 s  c caddr tr ,
+      is_init_state c caddr s0 ->
+      strat_subset_time addrs_env1 delta_env1 addrs_env2 delta_env2  s0 ->
+      UserLiquidatesNSteps miner_address addrs_usr delta_usr addrs_env2 delta_env2  caddr s0 s tr ->
+      UserLiquidatesNSteps miner_address addrs_usr delta_usr addrs_env1 delta_env1  caddr s0 s tr .
+  Proof.
+    intros * Hinit Hsbt_delta Hrc_itv.
+    eapply (env_mut miner_address addrs_usr delta_usr addrs_env2 delta_env2  caddr s0 
+    (fun s tr   (_ : envProgress_Mutual miner_address addrs_usr delta_usr addrs_env2 delta_env2  caddr s0 s tr ) =>  
+    envProgress_Mutual miner_address addrs_usr delta_usr addrs_env1 delta_env1  caddr s0 s tr )
+    (fun  s tr  (_ : UserLiquidatesNSteps miner_address addrs_usr delta_usr addrs_env2 delta_env2  caddr  s0 s tr ) => 
+    UserLiquidatesNSteps miner_address addrs_usr delta_usr addrs_env1 delta_env1  caddr s0 s tr )
+    );intros;subst;eauto.
+    - apply EPM_Base. assumption.
+    - eapply EPM_Step.
+      eauto.
+      intros.
+      assert (multiStratDrive miner_address addrs_env2 delta_env2 s0 s1 tr0 s' tr' n).
+      {
+        eapply multiStratDrive_subset_time;eauto.
+      }
+      specialize (H s' tr' n).
+      eapply H;eauto.
+    - eapply (EPM_Time miner_address addrs_usr delta_usr addrs_env1 delta_env1 caddr s0 s1 tr0  s' tr'  a1 a2);eauto.
+      unfold strat_subset_time in Hsbt_delta.
+      specialize (Hsbt_delta s1 tr0).
+      unfold acts_subset_time in Hsbt_delta.
+      destruct Hsbt_delta as [Hsbt_delta Hsbt_delta_time].
+      specialize (Hsbt_delta_time a2 e0 i0).
+      unfold acts_subset in Hsbt_delta.
+      intuition.
+    - eapply EPM_Turn;eauto.
+      unfold strat_subset_time in Hsbt_delta.
+      specialize (Hsbt_delta s1 tr0).
+      unfold acts_subset_time in Hsbt_delta.
+      destruct Hsbt_delta as [Hsbt_delta Hsbt_delta_time].
+      specialize (Hsbt_delta_time a e i).
+      unfold acts_subset in Hsbt_delta.
+      intuition.
+    - eapply ULM_Base;eauto.
+    - eapply ULM_Step;eauto.
+    - eapply (ULM_Time miner_address addrs_usr delta_usr addrs_env1 delta_env1 caddr s0 s1 tr0  s' tr'  a1 a2);eauto.
+      unfold strat_subset_time in Hsbt_delta.
+      specialize (Hsbt_delta s1 tr0).
+      unfold acts_subset_time in Hsbt_delta.
+      destruct Hsbt_delta as [Hsbt_delta Hsbt_delta_time].
+      specialize (Hsbt_delta_time a2 e0 i0).
+      unfold acts_subset in Hsbt_delta.
+      intuition.
+    - eapply ULM_Turn;eauto.
+  Qed.
+
+  Lemma strat_liquid_Mono_usr_unchanging 
+      (addrs_usr: list Address) (delta_usr : strat miner_address addrs_usr) 
+      (addrs_env1: list Address)  (delta_env1 : strat miner_address addrs_env1) 
+      (addrs_env2: list Address)  (delta_env2 : strat miner_address addrs_env2) :
+    forall s0 c caddr, 
+      is_init_state c caddr s0 ->
+      strat_subset_time addrs_env1 delta_env1 addrs_env2 delta_env2  s0->
+      strat_liquidity miner_address addrs_usr delta_usr  addrs_env2 delta_env2 c caddr  s0 ->
+      strat_liquidity miner_address addrs_usr delta_usr  addrs_env1 delta_env1 c caddr  s0.
+  Proof.
+    intros * Hinit Hstrat_refines Hliq_delta2.
+    unfold strat_liquidity in *.
+    intros Hwell_sys * Hrc_itv.
+    specialize(Hliq_delta2 Hinit tr s' tr').
+    assert (interleavedExecution miner_address addrs_usr delta_usr addrs_env2 delta_env2  s0 s0
+    tr Tusr s' tr').
+    eapply interleavedExecution_mono_incl_usr_unchanging_time;eauto.
+    specialize (Hliq_delta2 H).
+    decompose_exists.
+    eapply userLiquidatesNSteps_incl_usr_unchanging in Hliq_delta2;eauto.
+  Qed.
+
+End Monotonicity.
